# Section 10.3

### 1. $1+\frac13+\frac19+\frac1{27}+...$

- $\displaystyle\sum_{k=0}^{\infty} (\frac13)^k$

- $r = \frac13$

- $a = 1$

- $s = \frac{a}{1-r}$

**Answer:**

$\displaystyle\sum_{k=0}^{\infty} (\frac13)^k = \frac32$

---

### 2. $1+\frac23+\frac49+\frac8{27}+...$

- $\displaystyle\sum_{k=0}^{\infty} (\frac23)^k$

- $r = \frac23$

- $a = 1$

- $s = \frac{a}{1-r}$

**Answer:**

$\displaystyle\sum_{k=0}^{\infty} (\frac23)^k = 3$

---

### 3. $\frac18+\frac1{16}+\frac1{32}+\frac{1}{64}+...$

- $\displaystyle\sum_{k=0}^{\infty} (\frac12)^{k+3}$

- $r = \frac12$

- $a = \frac18$

- $s = \frac{a}{1-r}$

**Answer:**

$\displaystyle\sum_{k=0}^{\infty} (\frac12)^{k+3} = \frac14$

---

### 4. $1-\frac12+\frac1{4}-\frac1{8}+\frac{1}{16}-...$

- $\displaystyle\sum_{k=0}^{\infty} (-\frac12)^{k}$

- $r = -\frac12$

- $a = 1$

- $s = \frac{a}{1-r}$

**Answer:**

$\displaystyle\sum_{k=0}^{\infty} (-\frac12)^{k} = \frac23$

---

### 5. $-\frac23+\frac4{9}-\frac8{27}+...$

- $\displaystyle\sum_{k=0}^{\infty} (-\frac23)^{k+1}$

- $r = -\frac23$

- $a = -\frac23$

- $s = \frac{a}{1-r}$

**Answer:**

$\displaystyle\sum\_{k=0}^{\infty} (-\frac23)^{k+1} = -\frac25$

---

### 6. $1+\frac1{e}+\frac1{e^2}+\frac1{e^3}+...$

- $\displaystyle\sum_{k=0}^{\infty} (\frac1e)^{k}$

- $r = \frac1e$

- $a = 1$

- $s = \frac{a}{1-r}$

- $s = (\frac{e}{e}-\frac1e)^{-1}$

**Answer:**

$\displaystyle\sum_{k=0}^{\infty} (\frac1e)^{k} = \frac{e}{e-1}$

---

### 8. A ball is thrown 10 feet straight up into the air, and on each bounce, it rebounds to 60% of its previous height.

#### (a) How far does the ball travel (up and down) during its n th bounce.

#### (b) Use a sum to represent the total distance traveled by the ball.

#### \(c\) Find the total distance traveled by the ball

<br>

- $10 + 6 +...$

- $\displaystyle\sum_{k=0}^{\infty} 10 \times \Big(\frac{3}{5}\Big)^{k}$

- $r = \frac{3}{5}$

- $a = 10$

- $s = \frac{a}{1-r}$

**Answer:**

- $\displaystyle\sum_{k=0}^{\infty} 10 \times \Big(\frac{3}{5}\Big)^{k} = 25$

---

### 11. The mathematical diet you are following says you can eat "half of whatever is on the plate," so first you bite off one half of the cake and put the other half back on the plate. Then you pick up the remaining half from the plate (itâ€™s "on the plate"), bite off half of that, and return the rest to the plate. And you continue this silly process of picking up the piece from the plate, biting off half, and returning the rest to the plate

#### (a) Represent the total amount you eat as a series

#### (b) How much of the cake is left after 1 bite, 2 bites, n bites?

#### \(c\) "Eventually," how much of the cake do you eat?

<br>

- $\frac12 + \frac14 + \frac18 + ...$

- $\displaystyle\sum_{k=0}^{\infty} (\frac12)^{k+1}$

- $r = \frac{1}{2}$

- $a = \frac12$

- $s = \frac{a}{1-r}$

**Answer:**

$\displaystyle\sum_{k=0}^{\infty} (\frac12)^{k+1} = 1$

---

### 18. Represent the repeating decimals $0.\bar{6}$ and $0.\overline{63}$ as geometric series and find the value of each series as a simple fraction

<br>

- $\displaystyle\sum_{k=0}^{\infty} \frac{6}{10^{k+1}}$

- $r = \frac{1}{10}$

- $a = \frac{6}{10}$

- $s = \frac{a}{1-r}$

- $\displaystyle\sum_{k=0}^{\infty} \frac{63}{100^{k+1}}$

- $r = \frac{1}{100}$

- $a = \frac{63}{100}$

- $s = \frac{a}{1-r}$

**Answer:**

$\displaystyle\sum_{k=0}^{\infty} \frac{6}{10^{k+1}} = \frac23$

and

$\displaystyle\sum_{k=0}^{\infty} \frac{63}{100^{k+1}} = \frac{7}{11}$

---

### 33. One student thought the formula was $1+x+x^2+x^3+... = \frac{1}{1-x}$ The second student said "That can't be right. If we replace $x$ with $2$, then the formula says the sum of the positive numbers $1+2+4+8+...$ is a negative number $\frac{1}{1-2}=-1$" Who is right? Why?

<br>

**Answer:**

For the formula to be used $|r| >1 \space$ **must** be true and in the case of $x=2$ it is not, so the first student is correct the and second student is agruing under a false assumption. If $x=2$ then the series diverges.

---
