# Section 10.6

### 17. $\displaystyle \sum_{n=1}^{\infty}(-1)^{n+1}\frac{1}{n+5}$

- [x] $a_n>0$
- [x] $a_n>a_{n+1}$
- [x] $\displaystyle \lim_{n\to\infty} a_n=0$

**Answer:**

we can conclude that the series converges

---

### 18. $\displaystyle \sum_{n=2}^{\infty}(-1)^{n+1}\frac{1}{\ln(n)}$

- [x] $a_n>0$
- [x] $a_n>a_{n+1}$
- [ ] $\displaystyle \lim_{n\to\infty} a_n=0$

**Answer:**

we can conclude that the series diverges

---

### 19. $\displaystyle \sum_{n=1}^{\infty}(-1)^{n+1}\frac{n}{n^2+3}$

- [x] $a_n>0$
- [ ] $a_n>a_{n+1}$
- [x] $\displaystyle \lim_{n\to\infty} a_n=0$

**Answer:**

we can conclude that the series diverges

---

### 20. $\displaystyle \sum_{n=5}^{\infty}(-1)^{n+1}(0.99)^{n+1}$

- [x] $a_n>0$
- [x] $a_n>a_{n+1}$
- [x] $\displaystyle \lim_{n\to\infty} a_n=0$

**Answer:**

we can conclude that the series converges

---

### 21. $\displaystyle \sum_{n=1}^{\infty}(-1)^{n}\frac{|n+3|}{|n+7|}$

- [x] $a_n>0$
- [ ] $a_n>a_{n+1}$
- [ ] $\displaystyle \lim_{n\to\infty} a_n=0$

**Answer:**

we can conclude that the series diverges

---

# Section 10.7

### 1. $\displaystyle \sum_{n=1}^{\infty}(-1)^{n}\frac{1}{n+2}$

- [ ] $n^P ; P > 1$

- [x] $a_n>0$
- [x] $a_n>a_{n+1}$
- [x] $\displaystyle \lim_{n\to\infty} a_n=0$

**Answer:**

we can conclude that the series conditionally converges

---

### 2. $\displaystyle \sum_{n=1}^{\infty}(-1)^{n+1}\frac{1}{\sqrt{n}}$

- [ ] $n^P ; P > 1$

- [x] $a_n>0$
- [x] $a_n>a_{n+1}$
- [x] $\displaystyle \lim_{n\to\infty} a_n=0$

**Answer:**

we can conclude that the series conditionally converges

---

### 3. $\displaystyle \sum_{n=1}^{\infty}(-1)^{n+1}\frac{5}{n^3}$

- [x] $n^P ; P > 1$

- [x] $a_n>0$
- [x] $a_n>a_{n+1}$
- [x] $\displaystyle \lim_{n\to\infty} a_n=0$

**Answer:**

we can conclude that the series absolutely converges

---

### 4. $\displaystyle \sum_{n=1}^{\infty}(-1)^{n}\frac{1}{2+\ln(n)}$

- [ ] $n^P ; P > 1$

- [x] $a_n>0$
- [x] $a_n>a_{n+1}$
- [x] $\displaystyle \lim_{n\to\infty} a_n=0$

**Answer:**

we can conclude that the series conditionally converges

---

### 5. $\displaystyle \sum_{n=1}^{\infty}(-1)^{n+1}\frac{1}{2^n}$

- [x] $n^P ; P > 1$

- [x] $a_n>0$
- [x] $a_n>a_{n+1}$
- [x] $\displaystyle \lim_{n\to\infty} a_n=0$

**Answer:**

we can conclude that the series absolutely converges

---

### 6. $\displaystyle \sum_{n=1}^{\infty}(-1)^{n+1}\frac{1}{2^{-n}}$

- [ ] $n^P ; P > 1$

- [ ] $a_n>0$
- [ ] $a_n>a_{n+1}$
- [ ] $\displaystyle \lim_{n\to\infty} a_n=0$

**Answer:**

we can conclude that the series diverges

---

### 7. $\displaystyle \sum_{n=1}^{\infty}(-1)^{n}\frac{1}{n^2}$

- [x] $n^P ; P > 1$

- [x] $a_n>0$
- [x] $a_n>a_{n+1}$
- [x] $\displaystyle \lim_{n\to\infty} a_n=0$

**Answer:**

we can conclude that the series absolutely converges

---

### 8. $\displaystyle \sum_{n=1}^{\infty}(-1)^{n+1}\frac{1}{3+n^2}$

- [x] $n^P ; P > 1$

- [x] $a_n>0$
- [x] $a_n>a_{n+1}$
- [x] $\displaystyle \lim_{n\to\infty} a_n=0$

**Answer:**

we can conclude that the series absolutely converges

---

### 9. $\displaystyle \sum_{n=1}^{\infty}(-1)^{n+1}\frac{\ln(n)}{n}$

- [ ] $n^P ; P > 1$

- [x] $a_n>0$
- [x] $a_n>a_{n+1}$
- [ ] $\displaystyle \lim_{n\to\infty} a_n=0$

**Answer:**

we can conclude that the series diverges

---
