# Section 6.0

### 1. $y'+3y=6;\space y=e^{-3x}+2$

- $y'= -3e^{-3x}$
- $-3e^{-3x}+3(e^{-3x}+2)=6$

**Answer:**

- [x] correct solution

---

### 2. $y'-2y=8;\space y=e^{2x}-4$

- $y'= 2e^{2x}$
- $2e^{2x}-2(e^{2x}-4)=8$

**Answer:**

- [x] correct solution

---

### 3. $y''-y'+y=x^2;\space y=x^2+2x$

- $y'= 2x+2$
- $y''= 2$
- $2-(2x+2)+(x^2+2x)=x^2$
- $x^2+(2x-2x)+(2-2)=x^2$

**Answer:**

- [x] correct solution

---

### 4. $3y''+y'+y=x^2-4x;\space y=x^2-6x$

- $y'= 2x-6$
- $y''= 2$
- $3(2)+(2x-6)+(x^2-6x)=x^2-4x$
- $x^2+(-6x+2x)+(6-6)=x^2-4x$

**Answer:**

- [x] correct solution

---

### 5. $xy'-3y=x^2;\space y=7x^3-x^2$

- $y'= 21x^2-2x$
- $x(21x^2-2x)-3(7x^3-x^2)=x^2$
- $(21x^3-21x^3)+3x^2-2x^2=x^2$

**Answer:**

- [x] correct solution

---

### 6. $xy''-y'=3;\space y=x^2-3x+5$

- $y'= 2x-3$
- $y''= 2$
- $x(2)-(2x-3)=3$
- $(2x-2x)+3=3$

**Answer:**

- [x] correct solution

---

### 7. $y'+y=e^x;\space y=\frac12e^x+2e^{-x}$

- $y'= \frac12e^x-2e^{-x}$
- $\frac12e^x-2e^{-x}+(\frac12e^x+2e^{-x})=e^x$
- $\frac12e^x+\frac12e^x+(2e^{-x}-2e^{-x})=e^x$

**Answer:**

- [x] correct solution

---

### 8. $y''+25y=0;\space y=\sin(5x)+2\cos(5x)$

- $y'= 5\cos(5x)-10\sin(5x)$
- $y''= -25\sin(5x)-50\cos(5x)$
- $-25\sin(5x)-50\cos(5x)+25(\sin(5x)+2\cos(5x))=0$
- $-25\sin(5x)-50\cos(5x)+25\sin(5x)+50\cos(5x)=0$

**Answer:**

- [x] correct solution

---

### 9. $y'=-\frac{x}y;\space y=\sqrt{7-x^2}$

- $y'=\frac12(7-x^2)^{-1/2}\times-2x$
- $y'=-\frac{x}{\sqrt{7-x^2}}$
- $-\frac x{\sqrt{7-x^2}} = -\frac x{\sqrt{7-x^2}}$

**Answer:**

- [x] correct solution

---

### 10. $y'=x-y;\space y=x-1+2e^{-x}$

- $y'=-2e^x+1$
- $-2e^x+1=x-(x-1+2e^{-x})$
- $-2e^x+1=1-2e^{-x}$

**Answer:**

- [x] correct solution

---

### 32. $y'=x-e^x;\space y(0)=3$

- $y=\frac12x^2-e^x+c$
- $3=\frac12(0)^2-e^0+c$
- $c=4$

**Answer:**

$y=\frac12x^2-e^x+4$

---

### 33. $y'=\frac3x;\space y(1)=2$

- $y=3\ln|x|+c$
- $2=3\ln|1|+c$
- $c=2$

**Answer:**

$y=3\ln(x)+2$

---

### 34. $xy'=1;\space y(e)=7$

- $y'=\frac1x$
- $y=\ln|x|+c$
- $7=\ln|e|+c$
- $c=6$

**Answer:**

$y=\ln|x|+6$

---

### 35. $y'=6e^{2x};\space y(0)=1$

- $y=3e^{2x}+c$
- $1=3e^0+c$
- $c=-2$

**Answer:**

$y=3e^{2x}-2$

---

### 36. $y'=36(3x-2)^2;\space y(1)=8$

- $u=3x-2$
- $du=3$
- $y=4(3x-2)^3+c$
- $8=4(3(1)-2)^3+c$
- $c=4$

**Answer:**

$y=4(3x-2)^3+4$

---

### 37. $y'=(x)\sin(x^2);\space y(0)=3$

- $u=x^2$
- $du=2x$
- $y=-\frac12\cos(x^2)+c$
- $3=-\frac12\cos(0)+c$
- $c=3\frac12$

**Answer:**

$y=-\frac12\cos(x^2)+3\frac12$

---

### 38. $y'=6x^{-2};\space y(1)=2$

- $y=-6x^{-1}+c$
- $2=-6+c$
- $c=8$

**Answer:**

- $y=-6x^{-1}+8$

---

### 45. $dy=(A-By)\space dt;\space y=\frac{A}B-Ce^{-Bt}$

- $y'=BCe^{-Bt}$
- $BCe^{-Bt}=(A-B(\frac{A}B-Ce^{-Bt}))$
- $BCe^{-Bt}=(A-A)+BCe^{-Bt}$

**Answer:**

- [x] correct solution

---
