# Section 8.4

### 1. $\frac{7x+2}{x(x+1)}$

- $7x+2=A(x+1)+Bx$
- $\let x=0 7(x)+2=A(x+1)+B(x)$
- $A=2$
- $7(-1)+2=A(-1+1)+B(-1)$
- $B=5$

**Answer:**

- $f(x)=\frac{2}{x}+\frac{5}{x+1}$

---

### 2. $\frac{7x+9}{(x+3)(x-1)}$

- $7x+9=A(x-1)+B(x+3)$

- $7(-3)+9=A(-3-1)+B(-3+3)$
- $A=3$

- $7(1)+9=A(1-1)+B(1+3)$
- $B=4$

**Answer:**

- $f(x)=\frac{3}{x+3}+\frac{4}{x-1}$

---

### 3. $\frac{11x+25}{x^2+9x+8}$

- $\frac{11x+25}{(x+8)(x+1)}$
- $11x+25=A(x+1)+B(x+8)$

- $11(-8)+25=A(-8+1)+B(-8+8)$
- $A=9$

- $11(-1)+25=A(-1+1)+B(-1+8)$
- $B=2$

**Answer:**

- $f(x)=\frac{9}{x+8}+\frac{2}{x+1}$

---

### 4. $\frac{3x+7}{x^2-1}$

- $\frac{3x+7}{(x+1)(x-1)}$
- $3x+7=A(x-1)+B(x+1)$

- $3(-1)+7=A(-1-1)+B(-1+1)$
- $A=-2$

- $3(1)+7=A(1-1)+B(1+1)$
- $B=5$

**Answer:**

- $f(x)=\frac{-2}{x+1}+\frac{5}{x-1}$

---

### 13. $\int\frac{3x+13}{(x+2)(x-5)}dx$

- $3x+13=A(x-5)+B(x+2)$

- $3(-2)+13=A(-2-5)+B(-2+2)$
- $A=-1$

- $3(5)+13=A(5-5)+B(5+2)$
- $B=4$

- $f(x)=\frac{-1}{x+2}+\frac{4}{x-5}$

- $F(x) = -\ln(x+2)+4\ln(x-5) + C$

**Answer:**

- $F(x) = -\ln(x+2)+4\ln(x-5) + C$

---

### 14. $\int\frac{2x+11}{(x-7)(x-2)}dx$

- $2x+11=A(x-7)+B(x-2)$

- $2(7)+11=A(7-2)+B(7-7)$
- $A=5$

- $2(2)+11=A(2-7)+B(2-2)$
- $B=-3$

- $f(x)=\frac{5}{x-7}+\frac{-3}{x-2}$

- $F(x) = 5\ln(x-7)-3\ln(x-2) + C$

**Answer:**

- $F(x) = 5\ln(x-7)-3\ln(x-2) + C$

---

### 15. $\int_{2}^{5}\frac{2}{(x^2-1)}dx$

- $\int_{2}^{5}\frac{2}{(x+1)(x-1)}dx$
- $2=A(x-1)+B(x+1)$

- $2=A(-1-1)+B(-1+1)$
- $A=-1$

- $2=A(1-1)+B(1+1)$
- $B=1$

- $f(x)=\frac{-1}{x+1}+\frac{1}{x-1}$

- $F(x) = -\ln(x+1)+\ln(x-1) + C$

- $-\ln|5+1|+\ln|5-1| - (-\ln|2+1|+\ln|2-1|) \Big|_{2}^{5}$

- $-\ln|6|+\ln|4| + \ln|3| - \ln|1| \Big|_{2}^{5}$

**Answer:**

- $-\ln|6|+\ln|4| + \ln|3| - \ln|1|$

---

### 26. $\int \frac{2x+5}{(x+1)^2} dx$

- $\int 2x\frac{1}{x+1} + 5\frac{1}{x+1}dx$

- $u = 2x$
- $du = 2$
- $v = \ln|x+1|$
- $dv = \frac{1}{x+1}$

- $F(x) = 2x(\ln|x+1|)-\int [2\ln|x+1|] + 5\ln|x+1| + C$

**Answer:**

- $F(x) = 2x(\ln|x+1|)-\int [2\ln|x+1|] + 5\ln|x+1| + C$

---

### 33.1. $\frac{7x+2}{x(x+1)}$

- $7x+2=A(x+1)+Bx$
- $\let x=0 7(x)+2=A(x+1)+B(x)$
- $A=2$
- $7(-1)+2=A(-1+1)+B(-1)$
- $B=5$

- $f(x)=\frac{2}{x}+\frac{5}{x+1}$

**Answer:**

- $f'(x) = \frac{-2}{x^2} - \frac{5}{(x+1)^2}$

- $f''(x) = \frac{4}{x^3} + \frac{10}{(x+1)^3}$

---

### 33.2. $\frac{7x+9}{(x+3)(x-1)}$

- $7x+9=A(x-1)+B(x+3)$

- $7(-3)+9=A(-3-1)+B(-3+3)$
- $A=3$

- $7(1)+9=A(1-1)+B(1+3)$
- $B=4$

- $f(x)=\frac{3}{x+3}+\frac{4}{x-1}$

**Answer:**

- $f'(x)=\frac{-3}{(x+3)^2} - \frac{4}{(x-1)^2}$
- $f''(x)=\frac{6}{(x+3)^3} + \frac{8}{(x-1)^3}$

---

### 34.1. $\frac{11x+25}{x^2+9x+8}$

- $\frac{11x+25}{(x+8)(x+1)}$
- $11x+25=A(x+1)+B(x+8)$

- $11(-8)+25=A(-8+1)+B(-8+8)$
- $A=9$

- $11(-1)+25=A(-1+1)+B(-1+8)$
- $B=2$

- $f(x)=\frac{9}{x+8}+\frac{2}{x+1}$

**Answer:**

- $f'(x)=\frac{-9}{(x+8)^2}-\frac{2}{(x+1)^2}$

- $f''(x)=\frac{18}{(x+8)^3}+\frac{4}{(x+1)^3}$

---

### 34.2. $\frac{3x+7}{x^2-1}$

- $\frac{3x+7}{(x+1)(x-1)}$
- $3x+7=A(x-1)+B(x+1)$

- $3(-1)+7=A(-1-1)+B(-1+1)$
- $A=-2$

- $3(1)+7=A(1-1)+B(1+1)$
- $B=5$

- $f(x)=\frac{-2}{x+1}+\frac{5}{x-1}$

**Answer:**

- $f'(x)=\frac{2}{(x+1)^2}-\frac{5}{(x-1)^2}$
- $f''(x)=\frac{-4}{(x+1)^3}+\frac{10}{(x-1)^3}$
