# Section 8.3

### 2. $\int xe^{-x}dx; \space u = x$

- $u = x$
- $du = dx$
- $v = -e^{-x}$
- $dv = e^{-x}dx$

- $x(-e^{-x})-\int -e^{-x}dx$
- $-xe^{-x}+\int e^{-x}dx$
- $-xe^{-x} - e^{-x} + C$

**Answer:**

- $-xe^{-x} - e^{-x} + C$

---

### 3. $\int x^4\ln(x)dx; \space dv = x^4dx$

- $u = ln(x)$
- $du = \frac1x$
- $v = \frac15x^5$
- $dv = x^4dx$

- $ln(x)\ * \frac15x^5-\int \frac15x^5(\frac1x)$
- $ln(x)\ * \frac15x^5-\frac1{25}x^5+C$

**Answer:**

- $ln(x)\ * \frac15x^5-\frac1{25}x^5+C$

---

### 7. $\int_{0}^{1} x*{e^{-3x}}dx$

- $u = x$
- $du = dx$
- $v = -\frac13e^{-3x}$
- $dv = e^{-3x}$

- $\frac{-x}3e^{-3x}- \int -\frac13e^{-3x}dx$
- $\frac{-x}3e^{-3x} - \frac19e^{-3x} +C$
- $\frac{-1}3e^{-3} - \frac19e^{-3} - (\frac{0}3e^{0} - \frac19e^{0})$
- $\frac{-1}3e^{-3} - \frac19e^{-3} + 1$

**Answer:**

- $\frac{-1}3e^{-3} - \frac19e^{-3} + 1$

---

### 8. $\int_{0}^{1} 10x*{e^{3x}}dx$

- $u = 10x$
- $du = 10dx$
- $v = \frac13e^{3x}$
- $dv = e^{3x}$

- $10x(\frac13e^{3x})- \frac{10}{3}\int e^{3x}dx$
- $10x(\frac13e^{3x})- 10 e^{3x} + C$

- $10(1)(\frac13e^{3(1)})- 10 e^{3(1)} - (10(0)(\frac13e^{3(0)})- 10 e^{3(0)})$

**Answer:**

- $10(\frac13e^{3})- 10 e^{3} + 10$

---

### 10. $\int_{0}^{\pi} 5x*\sin(2x)dx$

- $u = 5x$
- $du = 5dx$
- $v = -\frac12\cos(2x)$
- $dv = \sin(2x)dx$

- $5x(-\frac12\cos(2x))+\frac{5}{2}\int \cos(2x)dx$
- $5x(-\frac12\cos(2x))+5\sin(2x)$
- $5(1)(-\frac12\cos(2(1)))+5\sin(2(1)) - (5(0)(-\frac12\cos(2(0)))+5\sin(2(0)))$

**Answer:**

- $5(-\frac12\cos(2)+5\sin(2) - 5\sin(2))$

---

### 12. $\int 6x*\sin(x^2+1)dx$

- $u = 6x$
- $du = 6dx$
- $v = -\frac12\cos(2x)$
- $dv = \sin(x^2+1)dx$

- $6x(-\frac12\cos(2x))+\frac{6}{2}\int \cos(2x)dx$
- $6x(-\frac12\cos(2x))+6\sin(2x)$
- $6(1)(-\frac12\cos(2(1)))+6\sin(2(1)) - (6(0)(-\frac12\cos(2(0)))+6\sin(2(0)))$

**Answer:**

- $6(-\frac12\cos(2)+6\sin(2) - 6\sin(2))$

---

### 13. $\int 12x*\cos(3x^2)dx$

- $u = \cos(3x^2)$
- $du = (6x)\sin(3x^2)$
- $v = 6x^2$
- $dv = 12x$

- $\cos(3x^2)(6x^2)- \int 6x^2 (\cos(3x^2))$

**Answer:**

- $\cos(3x^2)(6x^2)- \int 6x^2 (\cos(3x^2))$

---

### 14. $\int x^2*\cos(x)dx$

- $u = x^2$
- $du = 2x \space dx$
- $v = \sin(x)$
- $dv = \cos(x)$

- $(x^2)(\sin(x)) - \int \sin(x)(2x)$

**Answer:**

- $(x^2)(\sin(x)) - \int \sin(x)(2x)$

---

### 15. $\int_{1}^{3} \ln(2x+5) dx$

- $u = 2x+5$
- $du = 2 \space dx$

**Answer:**

- $\textrm{unknown}$

---

### 16. $\int x^3\ln(5x) dx$

- $u = \ln(5x)$
- $du = \frac1{x}$
- $v = x^3$
- $dv = 3x^2 \space dx$

- $\ln(5x)x^3-\int x^3 \frac1x$
- $\ln(5x)x^3- \frac13 x^3 +C$

**Answer:**

- $\ln(5x)x^3- \frac13 x^3 +C$

---

### 18. $\int_{1}^{e} \sqrt{x} * \ln(x) dx$

- $u = \ln(x)$
- $du = \frac1{x}$
- $v = \sqrt{x}$
- $dv = \frac12 x^{-1/2} \space dx$

- $\ln(x)\sqrt{x}- \int \sqrt{x} \frac1x$
- $\ln(x)\sqrt{x}- \frac32 x^{3/2}$
- $\ln(e)\sqrt{e}- \frac32 e^{3/2} - (\ln(1)\sqrt{1}- \frac32 1^{3/2})$

**Answer:**

- $\ln(e)\sqrt{e}- \frac32 e^{3/2} - (\ln(1)\sqrt{1}- \frac32 1^{3/2})$

---

### 20. $\int_{1}^{e} \sqrt{x} * \ln(x) dx$

- $u = \ln(x)$
- $du = \frac1{x}$
- $v = \sqrt{x}$
- $dv = \frac12 x^{-1/2} \space dx$

- $\ln(x)\sqrt{x}- \int \sqrt{x} \frac1x$
- $\ln(x)\sqrt{x}- \frac32 x^{3/2}$
- $\ln(e)\sqrt{e}- \frac32 e^{3/2} - (\ln(1)\sqrt{1}- \frac32 1^{3/2})$

**Answer:**

- $\ln(e)\sqrt{e}- \frac32 e^{3/2} - (\ln(1)\sqrt{1}- \frac32 1^{3/2})$
